Changes based on Stewart's awesomeness

graphics.v
@@ -1,4 +1,10 @@
-Require Import ZArith String FMaps FMapAVL ExtrOcamlString.
+(* To DO: 1) Finish the draw line function 
+          in the section for interp on line 89
+          2) Think up different specifications that would be useful*)
+
+(* Let me know if you have any questions *)
+
+Require Import PArith String FMaps FMapAVL ExtrOcamlString.
 (*So sams idea is to idendify primatives that are live within the graphics functions and to verify everything with respect to those primatives*)
 
 
@@ -13,103 +19,198 @@ Inductive color: Type :=
 
 
 (* The type of a single pixel's location*)
-Module pixel_l:=  PairOrderedType Z_as_OT Z_as_OT.
-
+Module pixel_l:=  PairOrderedType Positive_as_OT Positive_as_OT.
+Definition point : Type := (positive * positive).
 
 (* This is the map that we can use to define the state 
-    hopefully i'm making it's type is sound*)
+    hopefully i'm making it's type soundly*)
 Module pix :=  FMapAVL.Make pixel_l.
 
-
 Definition pixtype := pix.t.
-
-
-
 Print pix.
+(*The state is a map and a screen size*)
 Record State :=
+  mkState
   {
-    screen_state : pix.t pixel_l.t;
-    screen_size : pixel_l.t;
+    screen_state : pix.t color;
+    screen_size : point;
   }.
 
-
-
-
-
-
-
-Open Scope Z_scope.
+Open Scope positive_scope.
 (* We should put in some notation to make the map easier  *)
 (*    to use but I think this is enough to get the general idea.*)
 Definition update (p : pixel_l.t) (pelet : color)
   (orig : pix.t color) : pix.t color := (pix.add p pelet) orig.
 
-Program Definition emptyST  := pix.add (0,0) White _.
+Program Definition emptyST  := pix.add (1,1) White _.
 Next Obligation.
   apply pix.empty.
   Defined.
 
 
-Program Definition p := update (1,2) Red _.
-Next Obligation.
-apply pix.empty.
-Defined.
+Program Definition p := update (1,2) Red emptyST.
 Print p.
 
 Definition p1 := pix.add (2,2) Blue p.
-Compute pix.find (1,0) p1.
+Compute pix.find (1,1) p1.
 
-
-
-
-
-(*The syntax of commands in the ocaml graphics library*)
 (* Maybe we need a state monad I don't 
    know where it would help currently
    Maybe when we define the semantics we just make it a function/
    relation that changes the state*)
-
-
-(* Definition open_graph : string -> unit. *)
-
 (*Function interp (s : state) (exp : g_com) : state*)
 
 (* We need two different functions like ocaml stuff and stuff that is in coq and a type class that could take and differentiate the two.*)
 
-Class graph_primitive (T :Type) (I : Type) :=
-  {
-    open_graph : T -> (*Or make this a string*) I -> T;
-    resize_window : T -> Z -> Z -> T;
-    plot : T -> Z -> Z -> T
-  }.
-
-Fixpoint 
-
-
-(* Axioms for essential functions*)
 
 Inductive g_com : Type :=
-| open_graph : string -> g_com
-| resize_window : Z -> Z  -> g_com
-| close_graph : unit -> unit -> g_com
-| plot : Z -> Z -> unit -> g_com
-| plots : list (Z * Z) -> unit -> g_com
-| moveto : Z -> Z -> unit -> g_com
-| lineto : Z -> Z -> g_com
-| draw_rect : Z -> Z -> Z -> Z -> unit -> g_com
+| open_graph : point -> g_com
+| resize_window : point  -> g_com
+(* | close_graph : unit -> unit -> g_com *)
+| plot : point -> point -> color -> g_com
+(* | plots : list (Z * Z) -> unit -> g_com *)
+(* | moveto : point -> unit -> g_com *)
+(* | lineto : point -> g_com *)
+(* Rec with the bottom left point followed by the top right.*)          
+| draw_rect : point -> point -> color -> g_com
 | seq : g_com -> g_com -> g_com.
 
 Notation "a ;; b" := (seq a b) (at level 50, left associativity).
 
+(*These are going to be the basic 
+  functions that we build everything from*)
+Class graphics_prims (T :Type) :=
+  mkGraphicsPrims
+    {
+      init_state : unit -> T;
+      update_state : T -> point -> T;
+    (*This might have to take a color 
+      or maybe we need to have a current 
+      color in the state, feels more like the ocaml library*)
+      draw_pixel : T -> point -> color -> T;
+  }.
 
-(* Definition camel_string (s : char) : string :=  *)
-(*   let r := create (length s) in *)
-(*   Fixpoint fill pos : string := "". *)
+Section interp.
+  Context {T : Type} `{graphics_prims T}.
+
+  Definition interp_draw_line (t : T) (c : color)
+                                (p1 p2 : point) : T :=
+    draw_pixel t p1 c. (* need to make this actually draw a line 
+                          seems like a david thing*)
+  Fixpoint interp (t : T) (e : g_com) : T :=
+    match e with
+    | open_graph s_size => update_state t s_size
+    | resize_window s_size => update_state t s_size 
+    | plot p1 p2 c => interp_draw_line t c p1 p2
+    | draw_rect p1 p2 c =>
+      match p1, p2 with
+      | (x,y), (z,w) => (* lower-left and upper-right *)
+        let t1 := interp_draw_line t c (x,y) (x,w) in
+        let t2 := interp_draw_line t1 c (x,y) (z,y) in
+        let t3 := interp_draw_line t2 c (x,w) (z,w) in
+        let t4 := interp_draw_line t3 c (z,w) (z,y) in
+        t4
+      end
+    | seq g1 g2 => let st  := (interp t g1) in (interp st g1)
+    end.
+
+  Definition run (e : g_com) : T :=
+    interp (init_state tt) e.
+End interp.
+
+(*example Instances We would use the State that 
+         we defined above *)
 
 
-(* Axiom camel_string : Type -> Type. *)
-(* Axiom Y : Set -> Set -> Set. *)
-(* Extract Constant Y "'a" "'b" => " 'a*'b ". *)
+Record boolState : Type :=
+  mkStateB {
+      b : bool
+    }.
+
+Instance boolState_graphics_prims : graphics_prims boolState :=
+  mkGraphicsPrims
+    boolState
+    (fun (_:unit) => mkStateB false)
+    (fun s p => mkStateB (negb (b s)))
+    (fun s p c => mkStateB (negb (b s))).
+
+Open Scope positive_scope.
+
+Definition prog1 : g_com :=
+  draw_rect (1,2) (3,4) Red.
+
+Compute interp (init_state tt) prog1. 
+
+
+
+
+
+(* Example very tentatively modelling extraction into ocaml*)
+
+Axiom OGState : Type. (* OCaml graphics state *)(* Maybe makes this unit*)
+Axiom initial_OGState : OGState.
+
+(* OCaml graphics operations *)
+Definition ocaml_graphics_init : unit -> OGState :=
+  fun _ => initial_OGState.
+Definition ocaml_update_state : OGState -> point -> OGState :=
+  fun (s : OGState) p => s.
+Definition ocaml_draw_pixel : OGState -> point -> color -> OGState :=
+  fun (s:OGState) _ _ => s.
+
+Instance OGState_graphics_prims : graphics_prims OGState :=
+  mkGraphicsPrims
+    OGState
+    ocaml_graphics_init
+    ocaml_update_state
+    ocaml_draw_pixel.
+
+Require Import Ascii String.
+Definition s : string := "abc".
+Print s.
+
+Definition newline : ascii := ascii_of_pos 10.
+
+Require Import List. Import ListNotations.
+(* Maybe we can make a print function
+   that makes a string of the buffer*)
+Definition buf : string :=
+  String newline EmptyString ++ 
+  "                   .              " ++ String newline EmptyString ++
+  "                  ...             " ++ String newline EmptyString ++
+  "                 .....            " ++ String newline EmptyString ++
+  "                  ...             " ++ String newline EmptyString ++
+  "                   .              ".
+Compute buf.
+
+Extract Constant OGState => "unit".
+Extract Constant initial_OGState => "()".
+
+Extract Constant ocaml_graphics_init =>
+  "(fun _ -> Graphics.open_graph ())".
+Extract Constant ocaml_draw_pixel =>
+  "(fun _ p c -> 
+     let rec int_of_pos p = 
+       (match p with 
+         | XH -> 1
+         | XO p' -> 2 * int_of_pos p'
+         | XI p' -> (2 * int_of_pos p') + 1)
+     in 
+     Graphics.set_color c;
+     Graphics.draw_pixel """" (int_of_pos p))".
+
+Definition t : OGState := interp (init_state tt) prog1.
+
+Recursive Extraction t.
+Extraction "test.ml" t.
+
+
+
+
+
+
+
+
 
 
 (* Extract Constant camel_string "'x'"  => "let camel_string (s: char list) : string = *)
@@ -118,17 +219,13 @@ Notation "a ;; b" := (seq a b) (at level 50, left associativity).
 (* | [] -> r *)
 (* | c :: s -> r.[pos] <- c; fill (pos + 1) s *)
 (* in fill 0 s". *)
-Open Scope Z_scope.
-(*There are still commas between this stuff in program 1 but I guess we have the idea, and can hope gordan can fix this.*)
-
-(*So We should move on to actually modelling what these commands do in coq.*)
-
-Extract Inductive g_com => g_com [ "open_graph" "resize_window" "close_graph" "plot" "plots" "moveto" "lineto" "draw_rect" " "].
-
-Definition program1 : g_com := open_graph "200,300";;resize_window 200 300.
 
 
-Require Import ExtrOcamlZInt.
+(* Extract Inductive g_com => g_com [ "open_graph" "resize_window" "close_graph" "plot" "plots" "moveto" "lineto" "draw_rect" " "]. *)
+
+
+
+Require Import ExtrOcamlPosInt.
 Extraction Language Ocaml.
 
 Extraction "export.ml"  g_com program1.
